Broken here ...

Main.lean
@@ -1,7 +1,15 @@
 import RflFirstAttempt
 
-def main : IO Unit :=
-  IO.println s!"Hello, {hello}!"
+set_option diagnostics true
+
+def main : IO Unit := IO.println s!"Hello, {hello}!"
+
+def sub1 : Nat → Nat | Nat.zero => Nat.zero | Nat.succ x => x
+
+def is_nat_zero (n : Nat) : Prop := n = 0
+
+#eval is_nat_zero 0 -- True
+#eval is_nat_zero 1 -- False
 
 theorem two_eq_two : 2 = 2 := by exact rfl
 
@@ -9,10 +17,13 @@ theorem two_eq_two_b : 2 = 2 := by rfl
 
 example : 3 = 3 := by rfl
 
-def sub1 : Nat → Nat | Nat.zero => Nat.zero | Nat.succ x => x
-
 example : sub1 0 = 0 := by rfl
 
 theorem zero_eq_zero : sub1 0 = 0 := by rfl
 
 example : sub1 4 = 3 := by rfl
+
+example (x : Nat) : sub1 (Nat.succ x) = x := by rfl
+
+-- Example 4: Equality using a constant value
+example : is_nat_zero 0 = true := by rfl
